weakening of dead_nodes_go_quiet to make it provable

systems/chord-props/DeadNodesGoQuiet.v
@@ -12,30 +12,31 @@ Require Import Chord.SystemLemmas.
 Require Import Chord.LiveNodesStayLive.
 Require Import Chord.ValidPointersInvariant.
 
-Definition no_msgs_from (h : addr) (occ : occurrence) :=
-  forall dst,
-    channel (occ_gst occ) h dst = [].
+Require Import mathcomp.ssreflect.ssreflect.
 
-Definition no_msgs_from_dead_nodes (occ : occurrence) :=
-  forall h,
-    In h (failed_nodes (occ_gst occ)) ->
-    no_msgs_from h occ.
+Definition no_msgs_to_live_from (h : addr) (occ : occurrence) :=
+  forall dst, live_node (occ_gst occ) dst -> channel (occ_gst occ) h dst = [].
+
+Definition no_msgs_to_live_from_dead_nodes (occ : occurrence) :=
+  forall h, In h (failed_nodes (occ_gst occ)) -> no_msgs_to_live_from h occ.
+
+Definition msg_from_length (h : addr) (dst : addr) (occ : occurrence) : nat :=
+  length (channel (occ_gst occ) h dst).
 
 Lemma no_msgs_from_dead_nodes_elim :
-  forall occ,
-    no_msgs_from_dead_nodes occ ->
-    forall src dst,
-      In src (failed_nodes (occ_gst occ)) ->
-      channel (occ_gst occ) src dst = [].
+  forall occ, no_msgs_to_live_from_dead_nodes occ ->
+    (forall src, In src (failed_nodes (occ_gst occ)) ->
+     forall dst, live_node (occ_gst occ) dst ->
+     channel (occ_gst occ) src dst = []).
 Proof.
-  unfold no_msgs_from_dead_nodes, no_msgs_from.
+  unfold no_msgs_to_live_from_dead_nodes, no_msgs_to_live_from.
   auto.
 Qed.
 
 Lemma dead_nodes_go_quiet :
   forall ex,
     lb_execution ex ->
-    continuously (now no_msgs_from_dead_nodes) ex.
+    continuously (now no_msgs_to_live_from_dead_nodes) ex.
 Proof.
   (* measure argument on number of msgs from h with nonincreasing obvious,
      eventual drop due to the fact that any given message in the network is
